Nearly Succeed

ARINC653_MultiCore.thy
@@ -11,63 +11,85 @@ typedecl Message
 typedecl Port
 typedecl Core
 
-typedecl QChannel
+typedecl SampChannel
 
-datatype Domain = P Part | S Sched 
+datatype Domain = P Part | S Sched | F 
 
 record Config = c2s :: "Core \<Rightarrow> Sched"
                 p2s :: "Part \<Rightarrow> Sched set"
                 p2p :: "Port \<Rightarrow> Part"
-                chsrc :: "QChannel \<Rightarrow> Port"
-                chdest :: "QChannel \<Rightarrow> Port"  
-                chmax :: "QChannel \<Rightarrow> nat"
-  
+                scsrc :: "SampChannel \<Rightarrow> Port"
+                scdests :: "SampChannel \<Rightarrow> Port set"
+
 axiomatization conf::Config 
-  where bij_c2s: "bij (c2s conf)" 
-    and portsrc_disj: "\<forall>c1 c2. c1 \<noteq> c2 \<longrightarrow> (chsrc conf) c1 \<noteq> (chsrc conf) c2" 
-    and portdest_disj: "\<forall>c1 c2. c1 \<noteq> c2 \<longrightarrow> (chdest conf) c1 \<noteq> (chdest conf) c2" 
-    and portsrcdest_disj: "\<forall>c1 c2. (chsrc conf) c1 \<noteq> (chdest conf) c2"
-
-lemma inj_surj_c2s: "inj (c2s conf) \<and> surj (c2s conf)"
-  using bij_c2s by (simp add: bij_def) 
-
+  where bij_c2s: "bij (c2s conf)" and
+        surj_p2c: "surj (p2s conf)" and
+        scdests_not_emp: "\<forall>sc. (scdests conf) sc \<noteq> {}" and
+        port_disj: "range (scsrc conf) \<inter> (\<Union> (range (scdests conf))) = {}" and 
+        no_disconn_port: "\<forall>p. p\<in>range (scsrc conf) \<or> p\<in>\<Union> (range (scdests conf))" and
+        no_same_source: "inj (scsrc conf)" and  
+        no_same_dest: "(\<forall>ch1 ch2. ch1\<noteq>ch2 \<longrightarrow> 
+                         ((scdests conf) ch1 \<inter> (scdests conf) ch2) = {}) " and
+        bij_p2p: "inj (p2p conf)"
 
 definition gsch :: "Config \<Rightarrow> Core \<Rightarrow> Sched"
   where "gsch cfg k \<equiv> (c2s cfg) k"
 
+definition is_src_sampport :: "Config \<Rightarrow> Port \<Rightarrow> bool"
+  where "is_src_sampport sc p \<equiv> (p\<in>range (scsrc sc))"
+
+definition is_dest_sampport :: "Config \<Rightarrow> Port \<Rightarrow> bool"
+  where "is_dest_sampport sc p \<equiv> (p\<in>\<Union> (range (scdests sc)))"
+
+definition is_sampport :: "Config \<Rightarrow> Port \<Rightarrow> bool"
+  where "is_sampport sc p \<equiv> is_src_sampport sc p \<or> is_dest_sampport sc p"
+
 definition port_of_part :: "Config \<Rightarrow> Port \<Rightarrow> Part \<Rightarrow> bool"
   where "port_of_part sc po pa \<equiv> ((p2p sc) po = pa)"
+
+definition ch_srcsampport :: "Config \<Rightarrow> Port \<Rightarrow> SampChannel"
+  where "ch_srcsampport sc p \<equiv> SOME c. (scsrc sc) c = p"
+
+definition ch_destsampport :: "Config \<Rightarrow> Port \<Rightarrow> SampChannel"
+  where "ch_destsampport sc p \<equiv> SOME c. p\<in>((scdests sc) c)"
+
+lemma same_dest_sampport:
+  "(scdests conf) c1 = p1 \<Longrightarrow>
+   (scdests conf) c2 = p2 \<Longrightarrow>
+   p1 \<inter> p2 \<noteq> {} \<Longrightarrow>
+   c1 = c2 "
+  using no_same_dest by (meson inj_eq)
+
+lemma same_src_sampport:
+  "(scsrc conf) c1 = p1 \<Longrightarrow>
+   (scsrc conf) c2 = p2 \<Longrightarrow>
+   p1 = p2 \<Longrightarrow>
+   c1 = c2 "
+  using no_same_source by (meson inj_eq)
 
 definition par_ports :: "Config \<Rightarrow> Part \<Rightarrow> Port set"
   where "par_ports sc pa \<equiv> {p. port_of_part sc p pa}"
 
-definition is_src_qport :: "Config \<Rightarrow> Port \<Rightarrow> bool"
-  where "is_src_qport sc p \<equiv> (p\<in>range (chsrc sc))"
+lemma "pa\<noteq>pb \<Longrightarrow> par_ports conf pa \<inter> par_ports conf pb = {}"
+  using bij_p2p unfolding par_ports_def port_of_part_def by auto
 
-definition is_dest_qport :: "Config \<Rightarrow> Port \<Rightarrow> bool"
-  where "is_dest_qport sc p \<equiv> (p\<in>range (chdest sc))"
+definition par_sampling_ports :: "Config \<Rightarrow> Port set \<Rightarrow> Port set"
+  where "par_sampling_ports sc ps \<equiv> {p.  (is_sampport sc) p \<and> p\<in>ps}"
 
-definition ch_srcqport :: "Config \<Rightarrow> Port \<Rightarrow> QChannel"
-  where "ch_srcqport sc p \<equiv> SOME c. (chsrc sc) c = p"
+definition par_dest_sampling_ports :: "Config \<Rightarrow> Port set \<Rightarrow> Port set"
+  where "par_dest_sampling_ports sc ps \<equiv> {p.  (is_dest_sampport sc) p \<and> p\<in>ps}"
 
-definition ch_destqport :: "Config \<Rightarrow> Port \<Rightarrow> QChannel"
-  where "ch_destqport sc p \<equiv> SOME c. (chdest sc) c = p"
+definition par_src_sampling_ports :: "Config \<Rightarrow> Port set \<Rightarrow> Port set"
+  where "par_src_sampling_ports sc ps \<equiv> {p.  (is_src_sampport sc) p \<and> p\<in>ps}"
 
-definition par_src_qports :: "Config \<Rightarrow> Port set \<Rightarrow> Port set"
-where "par_src_qports sc ps \<equiv>  {p.  (is_src_qport sc) p \<and> p\<in>ps}"
+definition par_sampchan::"Config \<Rightarrow> Part \<Rightarrow> SampChannel set"
+where "par_sampchan sc pa \<equiv> (ch_srcsampport sc) ` (par_src_sampling_ports sc (par_ports sc pa)) \<union>
+                            (ch_destsampport sc) `(par_dest_sampling_ports sc (par_ports sc pa))"
 
-definition par_dest_qports :: "Config \<Rightarrow> Port set \<Rightarrow> Port set"
-  where "par_dest_qports sc ps \<equiv>  {p.  (is_dest_qport sc) p \<and> p\<in>ps}"
-
-definition par_qchan :: "Config \<Rightarrow> Part \<Rightarrow> QChannel set"
-  where "par_qchan sc pa \<equiv> (ch_srcqport sc) ` (par_src_qports sc (par_ports sc pa)) \<union> 
-                           (ch_destqport sc) ` (par_dest_qports sc (par_ports sc pa))"
-
-datatype PartMode = IDLE | READY | RUN
 
 definition ch_conn :: "Config \<Rightarrow> Part \<Rightarrow> Part \<Rightarrow> bool"
-  where "ch_conn cfg p1 p2 \<equiv> (\<exists>sch. (p2p cfg) ((chsrc cfg) sch) = p1 
-                                      \<and> (p2p cfg) ((chdest cfg) sch) = p2)"
+  where "ch_conn cfg p1 p2 \<equiv> (\<exists>sch p. (p2p cfg) ((scsrc cfg) sch) = p1 
+                                      \<and> p \<in> (scdests cfg) sch \<and> (p2p cfg) p = p2)"
 
 primrec ch_conn2 :: "Config \<Rightarrow> Domain \<Rightarrow> Domain \<Rightarrow> bool"
   where "ch_conn2 cfg (P p1) d2 = (case d2 of
@@ -81,12 +103,14 @@ primrec part_on_core :: "Config \<Rightarrow> Domain \<Rightarrow> Domain \<Righ
                                         S d22 \<Rightarrow> d22 \<in>((p2s cfg) d1))" |
         "part_on_core cfg (S d1) d2 = False"
 
-record State = cur :: "Sched \<Rightarrow> Part option"
-               qbuf :: "QChannel \<Rightarrow> Message list"
-               qbufsize :: "QChannel \<Rightarrow> nat"
-               partst :: "Part \<Rightarrow> PartMode"
 
-datatype EL = Core_InitE | ScheduleE | Send_Que_MessageE |  Recv_Que_MessageE
+datatype PartMode = IDLE | READY | RUN
+
+record State = cur :: "Sched \<Rightarrow> Part"
+               schan :: "SampChannel \<rightharpoonup> Message"
+               recv :: "Part \<rightharpoonup> Message"
+
+datatype EL = Core_InitE | ScheduleE | Write_Sampling_MessageE |  Read_Sampling_MessageE
 
 datatype parameter = Port Port | Message Message | Partition Part
 
@@ -94,14 +118,6 @@ type_synonym EventLabel = "EL \<times> (parameter list \<times> Core)"
 
 definition get_evt_label :: "EL \<Rightarrow> parameter list \<Rightarrow> Core \<Rightarrow> EventLabel" ("_ _ \<rhd> _" [0,0,0] 20)
   where "get_evt_label el ps k \<equiv> (el,(ps,k))"
-
-abbreviation "core_init_pre k \<equiv> \<lbrace>\<forall>p. c2s conf k \<in> p2s conf p \<longrightarrow> \<acute>partst p = IDLE\<rbrace>"
-abbreviation "core_init_rely k \<equiv> \<lbrace>(\<forall>p. c2s conf k \<in> p2s conf p \<longrightarrow> \<ordfeminine>partst p = \<ordmasculine>partst p)\<rbrace>"
-abbreviation "core_init_guar k \<equiv> \<lbrace>\<ordfeminine>cur= \<ordmasculine>cur \<and> \<ordfeminine>qbuf= \<ordmasculine>qbuf \<and> \<ordfeminine>qbufsize= \<ordmasculine>qbufsize 
-            \<and> (\<forall>p. c2s conf k \<in> p2s conf p \<longrightarrow> \<ordmasculine>partst p = IDLE \<and> \<ordfeminine>partst p = READY)
-            \<and> (\<forall>c p. c \<noteq> k \<and> c2s conf c \<in> p2s conf p \<longrightarrow> \<ordfeminine>partst  p = \<ordmasculine>partst p)\<rbrace> \<union> Id"
-
-
 
 definition Core_Init :: "Core \<Rightarrow> (EventLabel, Core, State) event" 
   where "Core_Init k \<equiv> 
@@ -114,72 +130,338 @@ definition Core_Init :: "Core \<Rightarrow> (EventLabel, Core, State) event"
 
 
 definition System_Init :: "Config \<Rightarrow> (State \<times> (EventLabel, Core, State) x)"
-  where "System_Init cfg \<equiv> (\<lparr>cur=(\<lambda>c. None ),
-                            qbuf = (\<lambda>c. []),
-                            qbufsize = (\<lambda>c. 0),
-                            partst = (\<lambda>p. IDLE)\<rparr>, 
+  where "System_Init cfg \<equiv> (\<lparr>cur = (\<lambda>c. SOME p. c\<in>(p2s cfg) p),
+                            schan = (\<lambda>c. None),
+                            recv = (\<lambda>c. None)\<rparr>, 
                             (\<lambda>k. Core_Init k))"
 
-definition Schedule :: "Core \<Rightarrow> Part \<Rightarrow> (EventLabel, Core, State) event" 
-  where "Schedule k p \<equiv> 
-    EVENT ScheduleE [Partition p] \<rhd> k 
-    WHERE
-       c2s conf k \<in> p2s conf p
-      \<and> (\<acute>partst p \<noteq> IDLE)
-      \<and> (\<acute>cur((c2s conf) k) = None 
-          \<or> c2s conf k \<in> p2s conf (the (\<acute>cur((c2s conf) k))))
+definition Schedule :: "Core  \<Rightarrow> (EventLabel, Core, State) event" 
+  where "Schedule k  \<equiv> 
+    EVENT ScheduleE [] \<rhd> k 
+    WHERE True
     THEN 
-      \<lbrace>True\<rbrace> IF (\<acute>cur((c2s conf) k) \<noteq> None) THEN 
-        \<lbrace>True\<rbrace> ATOMIC
-          \<lbrace>True\<rbrace> \<acute>partst := \<acute>partst(the (\<acute>cur ((c2s conf) k)) := READY);;
-          \<lbrace>True\<rbrace> \<acute>cur := \<acute>cur((c2s conf) k := None)
-               END
-      FI;; 
-     (\<lbrace>True\<rbrace> ATOMIC
-        \<lbrace>True\<rbrace> \<acute>cur := \<acute>cur((c2s conf) k := Some p);;
-        \<lbrace>True\<rbrace> \<acute>partst := \<acute>partst(p := RUN)
-      END)
+      \<lbrace>True\<rbrace> \<acute>cur := \<acute>cur((c2s conf) k := SOME p. (c2s conf) k \<in>(p2s conf) p) 
     END"
 
-definition Send_Que_Message :: "Core \<Rightarrow> Port \<Rightarrow> Message \<Rightarrow> (EventLabel, Core, State) event" 
-  where "Send_Que_Message k p m \<equiv> 
-    EVENT Send_Que_MessageE [Port p, Message m] \<rhd> k 
+definition Write_Sampling_Message :: "Core \<Rightarrow> Port \<Rightarrow> Message \<Rightarrow> (EventLabel, Core, State) event" 
+  where "Write_Sampling_Message k p m \<equiv> 
+    EVENT Write_Sampling_MessageE [Port p, Message m] \<rhd> k 
     WHERE
-      is_src_qport conf p
-      \<and> \<acute>cur ((c2s conf) k) \<noteq> None
-      \<and> port_of_part conf p (the (\<acute>cur ((c2s conf) k)))
+      is_src_sampport conf p
+      \<and> port_of_part conf p (\<acute>cur (gsch conf k))
     THEN
-      \<lbrace>is_src_qport conf p \<and> (\<exists>y. \<acute>cur ((c2s conf) k) = Some y) 
-      \<and> port_of_part conf p (the (\<acute>cur ((c2s conf) k)))\<rbrace> 
-      AWAIT \<acute>qbufsize (ch_srcqport conf p) < chmax conf (ch_srcqport conf p) THEN 
-        \<lbrace>is_src_qport conf p \<and> (\<exists>y. \<acute>cur ((c2s conf) k) = Some y) \<and> 
-        port_of_part conf p (the (\<acute>cur ((c2s conf) k)))\<rbrace> \<inter> \<lbrace>\<acute>qbufsize (ch_srcqport conf p) 
-        < chmax conf (ch_srcqport conf p)\<rbrace> 
-        \<acute>qbuf := \<acute>qbuf (ch_srcqport conf p := \<acute>qbuf (ch_srcqport conf p) @ [m]);;
-        \<lbrace>True\<rbrace> \<acute>qbufsize := \<acute>qbufsize (ch_srcqport conf p := \<acute>qbufsize (ch_srcqport conf p) + 1)
-      END
+      \<lbrace>is_src_sampport conf p \<and> port_of_part conf p (\<acute>cur (gsch conf k))\<rbrace> 
+      \<acute>schan := \<acute>schan (ch_srcsampport conf p := Some m)
     END"
 
-definition Recv_Que_Message :: "Core \<Rightarrow> Port \<Rightarrow> (EventLabel, Core, State) event" 
-  where "Recv_Que_Message k p \<equiv> 
-    EVENT Recv_Que_MessageE [Port p] \<rhd> k 
+definition Read_Sampling_Message :: "Core \<Rightarrow> Port \<Rightarrow> (EventLabel, Core, State) event" 
+  where "Read_Sampling_Message k p \<equiv> 
+    EVENT Read_Sampling_MessageE [Port p] \<rhd> k 
     WHERE
-      is_dest_qport conf p 
-      \<and> \<acute>cur ((c2s conf) k) \<noteq> None
-      \<and> port_of_part conf p (the (\<acute>cur ((c2s conf) k)))
-    THEN 
-      \<lbrace>True\<rbrace> AWAIT \<acute>qbufsize (ch_srcqport conf p) > 0 THEN 
-        \<lbrace>True\<rbrace> \<acute>qbuf := \<acute>qbuf (ch_srcqport conf p := tl (\<acute>qbuf (ch_srcqport conf p)));;
-        \<lbrace>True\<rbrace> \<acute>qbufsize := \<acute>qbufsize (ch_srcqport conf p := \<acute>qbufsize (ch_srcqport conf p) - 1)
-      END
+      is_dest_sampport conf p 
+      \<and> port_of_part conf p (\<acute>cur (gsch conf k))
+    THEN
+      \<lbrace>is_dest_sampport conf p \<and> port_of_part conf p (\<acute>cur (gsch conf k))\<rbrace> 
+      \<acute>recv := \<acute>recv ((p2p conf p) := (\<acute>schan (ch_destsampport conf p)))
     END"
+
+definition Core_Init_RGCond :: " (State) rgformula"
+  where "Core_Init_RGCond  \<equiv> RG[\<lbrace>True\<rbrace>,UNIV,Id,\<lbrace>True\<rbrace>]"
+
+definition Schedule_RGCond :: "Core  \<Rightarrow> (State) rgformula"
+  where "Schedule_RGCond k  \<equiv> 
+   (RG[\<lbrace>True\<rbrace>,
+       \<lbrace>True\<rbrace>, 
+       (\<lbrace>\<ordfeminine>schan= \<ordmasculine>schan \<and> \<ordfeminine>recv = \<ordmasculine>recv \<and> \<ordfeminine>cur (c2s conf k) = (SOME p. (c2s conf) k \<in>(p2s conf) p)
+          \<and> (\<forall>c. c \<noteq> k \<longrightarrow> \<ordfeminine>cur (c2s conf c) = \<ordmasculine>cur  (c2s conf c))\<rbrace> \<union> Id),
+       \<lbrace>True\<rbrace>])"
+
+definition Write_Sampling_Message_RGCond :: "Core \<Rightarrow> Port \<Rightarrow> Message \<Rightarrow> (State) rgformula"
+  where "Write_Sampling_Message_RGCond k p m \<equiv> (
+            RG[\<lbrace>True\<rbrace>,
+               \<lbrace>\<ordfeminine>cur (c2s conf k)= \<ordmasculine>cur (c2s conf k)\<rbrace>, 
+               (\<lbrace>\<ordfeminine>cur = \<ordmasculine>cur \<and> \<ordfeminine>recv = \<ordmasculine>recv \<and> 
+                (is_src_sampport conf p \<and> port_of_part conf p (\<ordmasculine>cur (c2s conf k)) \<longrightarrow>
+                 (\<forall>ch. ch \<noteq> ch_srcsampport conf p \<longrightarrow> \<ordfeminine>schan ch = \<ordmasculine>schan ch)) \<and> 
+                 (\<not> (is_src_sampport conf p \<and> port_of_part conf p (\<ordmasculine>cur (c2s conf k))) \<longrightarrow> 
+                  \<ordfeminine>schan  = \<ordmasculine>schan)\<rbrace>),
+               \<lbrace>True\<rbrace>])"
+
+definition Read_Sampling_Message_RGCond :: "Core \<Rightarrow> Port \<Rightarrow> (State) rgformula"
+  where "Read_Sampling_Message_RGCond k p \<equiv> 
+     RG[\<lbrace>True\<rbrace>,
+        \<lbrace>\<ordfeminine>cur (c2s conf k)= \<ordmasculine>cur (c2s conf k)\<rbrace>,
+        (\<lbrace>\<ordfeminine>cur= \<ordmasculine>cur \<and> \<ordfeminine>schan = \<ordmasculine>schan \<and> (\<forall>x. x \<noteq> \<ordmasculine>cur (gsch conf k) \<longrightarrow> \<ordfeminine>recv x = \<ordmasculine>recv x)\<rbrace>),
+        \<lbrace>True\<rbrace>]"
+
+definition Core_Init_RGF :: "Core \<Rightarrow> (EventLabel, Core, State) rgformula_e"
+  where "Core_Init_RGF k \<equiv> (Core_Init k, Core_Init_RGCond)"
+                                                  
+definition Schedule_RGF :: "Core \<Rightarrow> (EventLabel, Core, State) rgformula_e"
+  where "Schedule_RGF k \<equiv> (Schedule k, Schedule_RGCond k)"
+
+definition Write_Sampling_Message_RGF :: "Core \<Rightarrow> Port \<Rightarrow> Message \<Rightarrow> (EventLabel, Core, State) rgformula_e"
+  where "Write_Sampling_Message_RGF k p m \<equiv> (Write_Sampling_Message k p m, Write_Sampling_Message_RGCond k p m)"
+
+definition Read_Sampling_Message_RGF :: "Core \<Rightarrow> Port \<Rightarrow> (EventLabel, Core, State) rgformula_e"
+  where "Read_Sampling_Message_RGF k p  \<equiv> (Read_Sampling_Message k p, Read_Sampling_Message_RGCond k p)"
+
+definition EvtSys1_on_Core_RGF :: "Core \<Rightarrow> (EventLabel, Core, State) rgformula_es"
+  where "EvtSys1_on_Core_RGF k \<equiv> 
+            (rgf_EvtSys ({Schedule_RGF k} \<union>
+                          (\<Union>(p, m). {Write_Sampling_Message_RGF k p m}) \<union>
+                          (\<Union>p.{Read_Sampling_Message_RGF k p})),
+               RG[\<lbrace>True\<rbrace>,
+                  \<lbrace>\<ordfeminine>cur (c2s conf k)= \<ordmasculine>cur (c2s conf k)\<rbrace>,
+                  (\<lbrace>\<ordfeminine>cur= \<ordmasculine>cur \<or> \<ordfeminine>cur (c2s conf k) = (SOME p. (c2s conf) k \<in>(p2s conf) p)
+                                \<and> (\<forall>c. c\<noteq> k \<longrightarrow> \<ordfeminine>cur (c2s conf c) = \<ordmasculine>cur  (c2s conf c))\<rbrace>),
+                  \<lbrace>True\<rbrace>])"
+
+definition EvtSys_on_Core_RGF :: "Core \<Rightarrow> (EventLabel, Core, State) rgformula_es"
+  where "EvtSys_on_Core_RGF k  \<equiv> 
+          (rgf_EvtSeq (Core_Init_RGF k) (EvtSys1_on_Core_RGF k),
+           RG[\<lbrace>True\<rbrace>,
+              \<lbrace>\<ordfeminine>cur (c2s conf k)= \<ordmasculine>cur (c2s conf k)\<rbrace>,
+              (\<lbrace>\<ordfeminine>cur= \<ordmasculine>cur \<or> \<ordfeminine>cur (c2s conf k) = (SOME p. (c2s conf) k \<in>(p2s conf) p)
+                                \<and> (\<forall>c. c\<noteq> k \<longrightarrow> \<ordfeminine>cur (c2s conf c) = \<ordmasculine>cur  (c2s conf c))\<rbrace>),
+              \<lbrace>True\<rbrace>])"
+
+definition ARINCXKernel_Spec :: "(EventLabel, Core, State) rgformula_par"
+  where "ARINCXKernel_Spec \<equiv> (\<lambda>k. EvtSys_on_Core_RGF k)"
+
+definition Evt_sat_RG:: "(EventLabel, Core, State) event \<Rightarrow> (State) rgformula \<Rightarrow> bool" ("(_\<turnstile>_)" [60,60] 61)
+  where "Evt_sat_RG e rg \<equiv> \<turnstile> e sat\<^sub>e [Pre\<^sub>f rg, Rely\<^sub>f rg, Guar\<^sub>f rg, Post\<^sub>f rg]"
+
+lemma Core_Init_SatRG: "\<forall>k. Core_Init k \<turnstile> Core_Init_RGCond"
+  apply(simp add:Evt_sat_RG_def)
+  apply(rule allI)
+  apply(simp add:Core_Init_def)
+  apply(rule BasicEvt)
+    apply(simp add:body_def)
+    apply(rule Basic)
+    apply(simp add:Core_Init_RGCond_def Pre\<^sub>f_def Post\<^sub>f_def Guar\<^sub>f_def getrgformula_def)+
+    apply auto[1] 
+  apply(simp add:Core_Init_RGCond_def Pre\<^sub>f_def Post\<^sub>f_def Guar\<^sub>f_def Rely\<^sub>f_def getrgformula_def guard_def stable_def)
+  apply(simp add:Core_Init_RGCond_def Post\<^sub>f_def Rely\<^sub>f_def getrgformula_def stable_def)
+  apply(simp add:stable_def Core_Init_RGCond_def getrgformula_def Pre\<^sub>f_def)
+  apply(simp add:Core_Init_RGCond_def Guar\<^sub>f_def getrgformula_def stable_def)
+  done
+
+lemma inj_surj_c2s: "inj (c2s conf) \<and> surj (c2s conf)"
+  using bij_c2s by (simp add: bij_def) 
+
+lemma Sched_SatRG_help1: "{(s, t). t = s\<lparr>cur := (cur s)(c2s conf k := SOME p. c2s conf k \<in> p2s conf p)\<rparr>}
+         \<subseteq> \<lbrace>(\<forall>c. c \<noteq> k \<longrightarrow> \<ordfeminine>cur (c2s conf c) = \<ordmasculine>cur (c2s conf c))\<rbrace>" 
+  using inj_surj_c2s by (simp add: Collect_mono case_prod_beta' inj_eq)
+
+lemma Sched_SatRG: "\<forall>k. Schedule k \<turnstile> Schedule_RGCond k"
+  apply(simp add:Evt_sat_RG_def)  
+  apply(rule allI)
+  apply(simp add:Schedule_def)
+  apply(rule BasicEvt)
+    apply(simp add:body_def guard_def)
+    apply(rule Basic, simp)
+       apply(simp add:Schedule_RGCond_def Pre\<^sub>f_def Post\<^sub>f_def Guar\<^sub>f_def getrgformula_def)
+      apply(simp add:Schedule_RGCond_def Pre\<^sub>f_def Guar\<^sub>f_def getrgformula_def)
+  using Sched_SatRG_help1 apply fastforce
+     apply(simp add:stable_def Schedule_RGCond_def getrgformula_def Pre\<^sub>f_def)
+    apply(simp add:stable_def Schedule_RGCond_def getrgformula_def Post\<^sub>f_def)
+   apply(simp add:stable_def Schedule_RGCond_def getrgformula_def Pre\<^sub>f_def)
+  by (simp add:Schedule_RGCond_def getrgformula_def Guar\<^sub>f_def)
+
+lemma Write_Sampling_Message_SatRG: 
+  "\<forall>k p m. Write_Sampling_Message k p m \<turnstile> Write_Sampling_Message_RGCond k p m"
+  apply(simp add:Evt_sat_RG_def)
+  apply(rule allI)+
+  apply(simp add:Write_Sampling_Message_def)
+  apply(rule BasicEvt)
+    apply(simp add:body_def guard_def)
+    apply(rule Basic)
+        apply(simp add:Write_Sampling_Message_RGCond_def Pre\<^sub>f_def getrgformula_def)
+       apply(simp add:Write_Sampling_Message_RGCond_def Post\<^sub>f_def getrgformula_def)
+      apply (simp add: Write_Sampling_Message_RGCond_def Guar\<^sub>f_def getrgformula_def)
+  using gsch_def apply force
+     apply(simp add:stable_def Write_Sampling_Message_RGCond_def getrgformula_def Pre\<^sub>f_def Rely\<^sub>f_def gsch_def)
+    apply(simp add:stable_def Write_Sampling_Message_RGCond_def getrgformula_def Post\<^sub>f_def)
+   apply(simp add:stable_def Write_Sampling_Message_RGCond_def getrgformula_def Pre\<^sub>f_def Rely\<^sub>f_def)
+  by (simp add:Write_Sampling_Message_RGCond_def getrgformula_def Guar\<^sub>f_def)
+
+lemma Read_Sampling_Message_SatRG: "\<forall>k p. Read_Sampling_Message k p \<turnstile> Read_Sampling_Message_RGCond k p"
+  apply(simp add:Evt_sat_RG_def)
+  apply(rule allI)+ 
+  apply(simp add:Read_Sampling_Message_def)
+  apply(rule BasicEvt)
+    apply(simp add:body_def guard_def)
+    apply (rule Basic)
+        apply(simp add: Read_Sampling_Message_RGCond_def Rely\<^sub>f_def getrgformula_def stable_def gsch_def)
+       apply(simp add: Read_Sampling_Message_RGCond_def Post\<^sub>f_def Rely\<^sub>f_def getrgformula_def stable_def gsch_def)
+      apply(simp add: Read_Sampling_Message_RGCond_def Guar\<^sub>f_def getrgformula_def gsch_def)
+  using port_of_part_def apply force
+     apply (simp add: stable_def Read_Sampling_Message_RGCond_def Rely\<^sub>f_def getrgformula_def gsch_def)
+    apply (simp add: stable_def Read_Sampling_Message_RGCond_def Rely\<^sub>f_def Post\<^sub>f_def getrgformula_def gsch_def)
+   apply (simp add: stable_def Read_Sampling_Message_RGCond_def Rely\<^sub>f_def Pre\<^sub>f_def getrgformula_def gsch_def)
+  by (simp add: Read_Sampling_Message_RGCond_def getrgformula_def Guar\<^sub>f_def)
+
+lemma pre_all_true : "ef \<in> insert (Schedule_RGF k) ((\<Union>(p, m). {Write_Sampling_Message_RGF k p m}) 
+      \<union> (\<Union>p. {Read_Sampling_Message_RGF k p})) \<Longrightarrow> Pre\<^sub>e ef = \<lbrace>True\<rbrace>"
+  apply (case_tac "ef \<in> {(Schedule_RGF k)}")
+   apply (simp add: Schedule_RGF_def getrgformula_def Schedule_RGCond_def Pre\<^sub>e_def)
+  apply(case_tac " ef \<in>(\<Union>(p, m). {Write_Sampling_Message_RGF k p m})")
+   apply (simp add: Write_Sampling_Message_RGF_def getrgformula_def Write_Sampling_Message_RGCond_def Pre\<^sub>e_def)
+   apply force
+  apply (simp add: Read_Sampling_Message_RGF_def getrgformula_def Read_Sampling_Message_RGCond_def Pre\<^sub>e_def)
+  by force
+
+lemma post_all_true : "ef \<in> insert (Schedule_RGF k) ((\<Union>(p, m). {Write_Sampling_Message_RGF k p m}) 
+      \<union> (\<Union>p. {Read_Sampling_Message_RGF k p})) \<Longrightarrow> Post\<^sub>e ef = \<lbrace>True\<rbrace>"
+  apply (case_tac "ef \<in> {(Schedule_RGF k)}")
+   apply (simp add: Schedule_RGF_def getrgformula_def Schedule_RGCond_def Post\<^sub>e_def)
+  apply(case_tac " ef \<in>(\<Union>(p, m). {Write_Sampling_Message_RGF k p m})")
+   apply (simp add: Write_Sampling_Message_RGF_def getrgformula_def Write_Sampling_Message_RGCond_def Post\<^sub>e_def)
+   apply force
+  apply (simp add: Read_Sampling_Message_RGF_def getrgformula_def Read_Sampling_Message_RGCond_def Post\<^sub>e_def)
+  by force
+
+
+lemma EvtSys1_on_core_SatRG: 
+  "\<forall>k. \<turnstile> fst (EvtSys1_on_Core_RGF k) sat\<^sub>s 
+              [Pre\<^sub>f (snd (EvtSys1_on_Core_RGF k)), 
+               Rely\<^sub>f (snd (EvtSys1_on_Core_RGF k)), 
+               Guar\<^sub>f (snd (EvtSys1_on_Core_RGF k)), 
+               Post\<^sub>f (snd (EvtSys1_on_Core_RGF k))]"
+  apply(rule allI)
+  apply(simp add:EvtSys1_on_Core_RGF_def Pre\<^sub>f_def Rely\<^sub>f_def Guar\<^sub>f_def Post\<^sub>f_def getrgformula_def)
+  apply(rule EvtSys_h)
+         apply(clarify)
+         apply(case_tac "(a,b)\<in> {(Schedule_RGF k)}")
+  using Sched_SatRG Schedule_RGF_def Evt_sat_RG_def E\<^sub>e_def Pre\<^sub>e_def Rely\<^sub>e_def Guar\<^sub>e_def Post\<^sub>e_def 
+    Guar\<^sub>f_def Post\<^sub>f_def Pre\<^sub>f_def Rely\<^sub>f_def snd_conv fst_conv apply (metis singletonD)
+         apply(case_tac "(a,b)\<in>(\<Union>(p, m). {Write_Sampling_Message_RGF k p m})")
+          apply(clarify)
+  using Write_Sampling_Message_SatRG Write_Sampling_Message_RGF_def E\<^sub>e_def Pre\<^sub>e_def Rely\<^sub>e_def Guar\<^sub>e_def Post\<^sub>e_def
+    Guar\<^sub>f_def Post\<^sub>f_def Pre\<^sub>f_def Rely\<^sub>f_def snd_conv fst_conv Evt_sat_RG_def
+          apply (smt Abs_unit_cases empty_iff singletonD) 
+         apply(case_tac "(a,b)\<in>(\<Union>p. {Read_Sampling_Message_RGF k p})")
+          apply(clarify)
+  using Read_Sampling_Message_SatRG Read_Sampling_Message_RGF_def E\<^sub>e_def Pre\<^sub>e_def Rely\<^sub>e_def Guar\<^sub>e_def Post\<^sub>e_def
+    Guar\<^sub>f_def Post\<^sub>f_def Pre\<^sub>f_def Rely\<^sub>f_def snd_conv fst_conv Evt_sat_RG_def
+          apply (smt Abs_unit_cases empty_iff singletonD)
+         apply blast
+  
+        apply(clarify)
+        apply(case_tac "(a,b)\<in> {(Schedule_RGF k)}")
+         apply(simp add:Schedule_RGF_def Schedule_RGCond_def Pre\<^sub>e_def getrgformula_def)
+        apply(case_tac "(a,b)\<in>(\<Union>(p, m). {Write_Sampling_Message_RGF k p m})")
+         apply clarify
+         apply(simp add:Write_Sampling_Message_RGF_def Write_Sampling_Message_RGCond_def Pre\<^sub>e_def getrgformula_def)
+        apply(case_tac "(a,b)\<in>(\<Union>p. {Read_Sampling_Message_RGF k p})")
+         apply(clarify)
+         apply(simp add:Read_Sampling_Message_RGF_def Read_Sampling_Message_RGCond_def Pre\<^sub>e_def getrgformula_def)
+        apply blast
+  
+       apply(clarify)
+       apply(case_tac "(a,b)\<in> {(Schedule_RGF k)}")
+        apply(simp add:Schedule_RGF_def Schedule_RGCond_def Rely\<^sub>e_def getrgformula_def)
+       apply(case_tac "(a,b)\<in>(\<Union>(p, m). {Write_Sampling_Message_RGF k p m})")
+  apply clarify
+        apply(simp add:Write_Sampling_Message_RGF_def Write_Sampling_Message_RGCond_def Rely\<^sub>e_def getrgformula_def)
+       apply(case_tac "(a,b)\<in>(\<Union>p. {Read_Sampling_Message_RGF k p})")
+        apply(clarify)
+        apply(simp add:Read_Sampling_Message_RGF_def Read_Sampling_Message_RGCond_def Rely\<^sub>e_def getrgformula_def)
+       apply blast
+  
+      apply(clarify)
+      apply(case_tac "(a,b)\<in> {(Schedule_RGF k)}")
+       apply(simp add:Schedule_RGF_def Schedule_RGCond_def getrgformula_def Guar\<^sub>e_def) apply auto[1]
+      apply(case_tac "(a,b)\<in>(\<Union>(p, m). {Write_Sampling_Message_RGF k p m})")
+       apply(simp add:Write_Sampling_Message_RGF_def Write_Sampling_Message_RGCond_def getrgformula_def Guar\<^sub>e_def)
+      apply(case_tac "(a,b)\<in>(\<Union>p. {Read_Sampling_Message_RGF k p})")
+        apply(simp add:Read_Sampling_Message_RGF_def Read_Sampling_Message_RGCond_def getrgformula_def Guar\<^sub>e_def)
+       apply force
+      apply(clarify)
+     apply(case_tac "(a,b)\<in> {(Schedule_RGF k)}")
+      apply(simp add:Schedule_RGF_def Schedule_RGCond_def getrgformula_def Guar\<^sub>e_def)
+     apply(case_tac "(a,b)\<in>(\<Union>(p, m). {Write_Sampling_Message_RGF k p m})")
+      apply(simp add:Write_Sampling_Message_RGF_def Write_Sampling_Message_RGCond_def getrgformula_def Guar\<^sub>e_def)
+     apply(case_tac "(a,b)\<in>(\<Union>p. {Read_Sampling_Message_RGF k p})")
+      apply(simp add:Read_Sampling_Message_RGF_def Read_Sampling_Message_RGCond_def getrgformula_def Guar\<^sub>e_def)
+     apply blast
+
+    apply(clarify)
+    apply(case_tac "(a,b)\<in> {(Schedule_RGF k)}")
+     apply(case_tac "(a,b)\<in> {(Schedule_RGF k)}")
+      apply(simp add:Schedule_RGF_def Schedule_RGCond_def getrgformula_def Pre\<^sub>e_def)
+     apply(case_tac "(a,b)\<in>(\<Union>(p, m). {Write_Sampling_Message_RGF k p m})")
+      apply(simp add:Write_Sampling_Message_RGF_def Write_Sampling_Message_RGCond_def getrgformula_def Pre\<^sub>e_def)
+     apply(case_tac "(a,b)\<in>(\<Union>p. {Read_Sampling_Message_RGF k p})")
+      apply(simp add:Read_Sampling_Message_RGF_def Read_Sampling_Message_RGCond_def getrgformula_def Pre\<^sub>e_def)
+     apply blast
+    apply(case_tac "(a,b)\<in>(\<Union>(p, m). {Write_Sampling_Message_RGF k p m})")
+     apply(case_tac "(a,b)\<in> {(Schedule_RGF k)}")
+      apply(simp add:Schedule_RGF_def Schedule_RGCond_def getrgformula_def Pre\<^sub>e_def)
+     apply(case_tac "(a,b)\<in>(\<Union>(p, m). {Write_Sampling_Message_RGF k p m})")
+      apply(simp add:Write_Sampling_Message_RGF_def Write_Sampling_Message_RGCond_def getrgformula_def Pre\<^sub>e_def)
+     apply(case_tac "(a,b)\<in>(\<Union>p. {Read_Sampling_Message_RGF k p})")
+      apply(simp add:Read_Sampling_Message_RGF_def Read_Sampling_Message_RGCond_def getrgformula_def Pre\<^sub>e_def)
+     apply blast
+    apply(case_tac "(a,b)\<in>(\<Union>p. {Read_Sampling_Message_RGF k p})")
+     apply(case_tac "(a,b)\<in> {(Schedule_RGF k)}")
+      apply(simp add:Schedule_RGF_def Schedule_RGCond_def getrgformula_def Pre\<^sub>e_def)
+     apply(case_tac "(a,b)\<in>(\<Union>(p, m). {Write_Sampling_Message_RGF k p m})")
+      apply(simp add:Write_Sampling_Message_RGF_def Write_Sampling_Message_RGCond_def getrgformula_def Pre\<^sub>e_def)
+     apply(case_tac "(a,b)\<in>(\<Union>p. {Read_Sampling_Message_RGF k p})")
+      apply(simp add:Read_Sampling_Message_RGF_def Read_Sampling_Message_RGCond_def getrgformula_def Pre\<^sub>e_def)
+     apply blast
+     apply blast
+  using pre_all_true apply force
+   apply (simp add: Ann_PiCore_Hoare.stable_def)
+  by force
+
+
+lemma EvtSys_on_core_SatRG: 
+  "\<forall>k. \<turnstile> fst (EvtSys_on_Core_RGF k) sat\<^sub>s 
+              [Pre\<^sub>f (snd (EvtSys_on_Core_RGF k)), 
+               Rely\<^sub>f (snd (EvtSys_on_Core_RGF k)), 
+               Guar\<^sub>f (snd (EvtSys_on_Core_RGF k)), 
+               Post\<^sub>f (snd (EvtSys_on_Core_RGF k))]"
+  apply(rule allI)
+  apply(simp add:EvtSys_on_Core_RGF_def Pre\<^sub>f_def Rely\<^sub>f_def Guar\<^sub>f_def Post\<^sub>f_def getrgformula_def)
+  apply(rule EvtSeq_h)
+          apply(simp add:E\<^sub>e_def Core_Init_RGF_def Pre\<^sub>e_def Rely\<^sub>e_def Guar\<^sub>e_def Post\<^sub>e_def)
+  using Core_Init_SatRG getrgformula_def apply (simp add: Evt_sat_RG_def Guar\<^sub>f_def Post\<^sub>f_def Pre\<^sub>f_def Rely\<^sub>f_def) 
+  using EvtSys1_on_core_SatRG apply simp
+        apply(simp add:Core_Init_RGF_def Core_Init_RGCond_def Pre\<^sub>e_def getrgformula_def)
+       apply(simp add:EvtSys1_on_Core_RGF_def Post\<^sub>f_def getrgformula_def)
+      apply(simp add:Core_Init_RGF_def Core_Init_RGCond_def Rely\<^sub>e_def getrgformula_def)
+     apply(simp add:EvtSys1_on_Core_RGF_def Rely\<^sub>f_def getrgformula_def)
+    apply(simp add:Core_Init_RGF_def Core_Init_RGCond_def Guar\<^sub>e_def getrgformula_def) 
+    apply auto[1]
+   apply(simp add:EvtSys1_on_Core_RGF_def Core_Init_RGCond_def Guar\<^sub>f_def getrgformula_def)
+  by (simp add:EvtSys1_on_Core_RGF_def Core_Init_RGF_def Core_Init_RGCond_def Post\<^sub>e_def Pre\<^sub>f_def getrgformula_def)
+
+lemma spec_sat_rg: "\<turnstile> ARINCXKernel_Spec SAT [{s0}, {}, UNIV, UNIV]"
+  apply (rule ParallelESys)
+       apply(simp add:ARINCXKernel_Spec_def) using EvtSys_on_core_SatRG
+       apply (simp add: Guar\<^sub>e\<^sub>s_def Guar\<^sub>f_def Post\<^sub>e\<^sub>s_def Post\<^sub>f_def Pre\<^sub>e\<^sub>s_def Pre\<^sub>f_def Rely\<^sub>e\<^sub>s_def Rely\<^sub>f_def) 
+      apply(simp add:ARINCXKernel_Spec_def EvtSys_on_Core_RGF_def Pre\<^sub>e\<^sub>s_def getrgformula_def)
+     apply simp
+    apply(rule allI)+
+    apply(simp add:ARINCXKernel_Spec_def EvtSys_on_Core_RGF_def Guar\<^sub>e\<^sub>s_def Rely\<^sub>e\<^sub>s_def getrgformula_def)
+    apply (simp add: Collect_mono Id_fstsnd_eq)
+   apply simp+
+  done
+
+
+axiomatization s0 where s0_init: "s0 \<equiv> fst (System_Init conf)"
+axiomatization x0 where x0_init: "x0 \<equiv> snd (System_Init conf)"
+axiomatization C0 where C0_init: "C0 = (paresys_spec ARINCXKernel_Spec, s0, x0)"
 
 definition domevt :: "State \<Rightarrow> Core \<Rightarrow> (EventLabel, Core, State) event \<Rightarrow> Domain"
-  where "domevt s k e \<equiv>  
-                         (if (\<exists>p m. e = Send_Que_Message k p m )\<or>                             
-                             (\<exists>p. e = Recv_Que_Message k p) then
-                              P (the ((cur s) (gsch conf k)))
-                         else S (gsch conf k))"  (*for convenience, we also consider domain of other(undefined) event as the sched*)
+  where "domevt s k e \<equiv>  (if (\<exists>p m. e = Write_Sampling_Message k p m )\<or>                             
+                             (\<exists>p. e = Read_Sampling_Message k p) then
+                              P  ((cur s) (gsch conf k))
+                          else S (gsch conf k))"  
+      (*for convenience, we also consider domain of other(undefined) event as the sched*)
 
 definition exec_step :: "(EventLabel, Core, State, Domain) action \<Rightarrow> 
  ((EventLabel, Core, State) pesconf \<times> (EventLabel, Core, State) pesconf) set"
@@ -198,20 +480,26 @@ definition interf :: "Domain \<Rightarrow> Domain \<Rightarrow> bool" ("(_ \<lea
 definition noninterf1 :: "Domain \<Rightarrow> Domain \<Rightarrow> bool" ("(_ \<setminus>\<leadsto> _)" [70,71] 60)
   where "u \<setminus>\<leadsto> v \<equiv> \<not> (u \<leadsto> v)"
 
-axiomatization s0 where s0_init: "s0 \<equiv> fst (System_Init conf)"
 
 definition state_obs_sched :: "State \<Rightarrow> Sched \<Rightarrow> State"
   where "state_obs_sched s d \<equiv> s0\<lparr>cur:=(cur s0) (d:=(cur s) d)\<rparr>"
 
-definition state_obs_part :: "State \<Rightarrow> Part \<Rightarrow> State"
-  where "state_obs_part s p \<equiv> s0\<lparr>partst:=(partst s0) (p:=(partst s) p)\<rparr> "
 
-definition qbuf_obs_part :: "State \<Rightarrow> Part \<Rightarrow> (QChannel \<Rightarrow> Message list)"
-  where "q_obs_part s p \<equiv> (qbuf s) |` (par_qchan conf p)"
+definition schan_obs_part :: "State \<Rightarrow> Part \<Rightarrow> (SampChannel \<rightharpoonup> Message)"
+  where "schan_obs_part s p \<equiv> (schan s) |` (par_sampchan conf p)  "
+
+definition state_obs_part :: "State \<Rightarrow> Part \<Rightarrow> State"
+  where "state_obs_part s p \<equiv> s0\<lparr>schan := schan_obs_part s p, 
+                                 recv := (recv s0) (p := (recv s) p)\<rparr>"
 
 primrec state_obs :: "State \<Rightarrow> Domain \<Rightarrow> State"
   where "state_obs s (P p) = state_obs_part s p" |
         "state_obs s (S p) = state_obs_sched s p"
+
+lemma ch_destsampport_same : "\<lbrakk>schan_obs_part s1 d = schan_obs_part s2 d; port_of_part conf p d; 
+      is_dest_sampport conf p\<rbrakk> \<Longrightarrow> schan s1 (ch_destsampport conf p) = schan s2 (ch_destsampport conf p)"
+  apply (simp add: schan_obs_part_def par_dest_sampling_ports_def par_ports_def par_sampchan_def)
+  by (metis (mono_tags, lifting) Un_iff imageI mem_Collect_eq restrict_in)
 
 definition state_equiv :: "State \<Rightarrow> Domain \<Rightarrow> State \<Rightarrow> bool" ("(_ \<sim>_\<sim> _)" [70,69,70] 60)
   where "state_equiv s d t \<equiv> state_obs s d = state_obs t d"
@@ -224,6 +512,526 @@ lemma state_equiv_symmetric : "s \<sim> d \<sim> t \<Longrightarrow> t \<sim> d 
 
 lemma state_equiv_reflexive : "s \<sim> d \<sim> s"
   by (simp add:state_equiv_def)
+
+
+lemma neq_coreinit: "k1\<noteq>k2 \<Longrightarrow> Core_Init k1\<noteq>Core_Init k2" 
+  by (simp add:Core_Init_def get_evt_label_def)
+
+lemma neq_schedule: "k1\<noteq>k2 \<Longrightarrow> Schedule k1\<noteq>Schedule k2" 
+  by (simp add:Schedule_def get_evt_label_def)
+
+lemma neq_wrt_samp: "(k1\<noteq>k2 \<or> p1\<noteq>p2 \<or> m1\<noteq>m2) \<Longrightarrow> Write_Sampling_Message k1 p1 m1 \<noteq> Write_Sampling_Message k2 p2 m2" 
+  apply (clarsimp, simp add:Write_Sampling_Message_def) 
+  by (simp add:get_evt_label_def)
+
+lemma neq_rd_samp: "(k1\<noteq>k2 \<or> p1\<noteq>p2) \<Longrightarrow> Read_Sampling_Message k1 p1 \<noteq> Read_Sampling_Message k2 p2" 
+  apply (clarsimp, simp add:Read_Sampling_Message_def) 
+  by (simp add:get_evt_label_def)
+
+lemma neq_coreinit_sched: "Core_Init k1 \<noteq> Schedule k2"
+  by (simp add:Schedule_def Core_Init_def get_evt_label_def)
+
+lemma neq_coreinit_wrtsamp: "Core_Init k1 \<noteq> Write_Sampling_Message k2 p m"
+  by (simp add:Write_Sampling_Message_def Core_Init_def get_evt_label_def)
+
+lemma neq_coreinit_rdsamp: "Core_Init k1 \<noteq> Read_Sampling_Message k2 p"
+  by (simp add:Read_Sampling_Message_def Core_Init_def get_evt_label_def)
+
+lemma neq_sched_wrtsamp: "Schedule k1 \<noteq> Write_Sampling_Message k2 p m"
+  by (simp add:Write_Sampling_Message_def Schedule_def get_evt_label_def)
+
+lemma neq_sched_rdsamp: "Schedule k1 \<noteq> Read_Sampling_Message k2 p"
+  by (simp add:Read_Sampling_Message_def Schedule_def get_evt_label_def)
+
+lemma neq_wrtsamp_rdsamp: "Write_Sampling_Message k1 p1 m \<noteq> Read_Sampling_Message k2 p2"
+  by (simp add:Read_Sampling_Message_def Write_Sampling_Message_def get_evt_label_def)
+
+definition evtrgfset :: "((EventLabel, Core, State) event \<times> (State rgformula)) set"
+  where "evtrgfset \<equiv> (\<Union>k.{(Core_Init k, Core_Init_RGCond)})
+                  \<union> (\<Union>k.{(Schedule k, Schedule_RGCond k)})
+                  \<union> (\<Union>(k, p, m).{(Write_Sampling_Message k p m, Write_Sampling_Message_RGCond k p m)})
+                  \<union> (\<Union>(k, p).{(Read_Sampling_Message k p, Read_Sampling_Message_RGCond k p)})"
+
+lemma evtrgfset_eq_allevts_ARINCSpec: "all_evts ARINCXKernel_Spec = evtrgfset"
+  proof -
+    have "all_evts ARINCXKernel_Spec = (\<Union>k. all_evts_es (fst (ARINCXKernel_Spec k)))" 
+      by (simp add:all_evts_def)
+    then have "all_evts ARINCXKernel_Spec = (\<Union>k. all_evts_es (fst (EvtSys_on_Core_RGF k)))"
+      by (simp add:ARINCXKernel_Spec_def)
+    then have "all_evts ARINCXKernel_Spec = (\<Union>k. all_evts_es (rgf_EvtSeq (Core_Init_RGF k) (EvtSys1_on_Core_RGF k)))"
+      by (simp add:EvtSys_on_Core_RGF_def)
+    then have "all_evts ARINCXKernel_Spec = (\<Union>k. {Core_Init_RGF k} \<union> (all_evts_es (fst (EvtSys1_on_Core_RGF k))))"
+      by simp
+    then have "all_evts ARINCXKernel_Spec = (\<Union>k. {Core_Init_RGF k} \<union>
+                                                  ({Schedule_RGF k} \<union>
+                                                  (\<Union>(p, m). {Write_Sampling_Message_RGF k p m}) \<union>
+                                                  (\<Union>p.{Read_Sampling_Message_RGF k p}))
+                                             )"
+      by (simp add:Core_Init_RGF_def EvtSys1_on_Core_RGF_def)
+    then have "all_evts ARINCXKernel_Spec = (\<Union>k. {(Core_Init k, Core_Init_RGCond)} \<union>
+                                                  {(Schedule k, Schedule_RGCond k)} \<union>
+                                                  (\<Union>(p, m). {(Write_Sampling_Message k p m, Write_Sampling_Message_RGCond k p m)}) \<union>
+                                                  (\<Union>p.{(Read_Sampling_Message k p, Read_Sampling_Message_RGCond k p)})
+                                             )"
+      by (simp add: Core_Init_RGF_def Schedule_RGF_def Write_Sampling_Message_RGF_def Read_Sampling_Message_RGF_def)
+    moreover
+    have "(\<Union>k. {(Core_Init k, Core_Init_RGCond)} \<union>
+                {(Schedule k, Schedule_RGCond k)} \<union>
+                (\<Union>(p, m). {(Write_Sampling_Message k p m, Write_Sampling_Message_RGCond k p m)}) \<union>
+                (\<Union>p.{(Read_Sampling_Message k p, Read_Sampling_Message_RGCond k p)})
+           ) = 
+           (\<Union>k. {(Core_Init k, Core_Init_RGCond)}) \<union>
+           (\<Union>k. {(Schedule k, Schedule_RGCond k)}) \<union>
+           (\<Union>k. (\<Union>(p, m). {(Write_Sampling_Message k p m, Write_Sampling_Message_RGCond k p m)})) \<union>
+           (\<Union>k. (\<Union>p.{(Read_Sampling_Message k p, Read_Sampling_Message_RGCond k p)}))"
+      by auto
+    moreover
+    have "(\<Union>k. (\<Union>(p, m). {(Write_Sampling_Message k p m, Write_Sampling_Message_RGCond k p m)}))
+          = (\<Union>(k, p, m). {(Write_Sampling_Message k p m, Write_Sampling_Message_RGCond k p m)})" by blast
+    moreover
+    have "(\<Union>k. (\<Union>p.{(Read_Sampling_Message k p, Read_Sampling_Message_RGCond k p)}))
+          = (\<Union>(k,p).{(Read_Sampling_Message k p, Read_Sampling_Message_RGCond k p)})" by blast
+    ultimately show ?thesis using evtrgfset_def by simp
+  qed
+
+definition evtrgffun :: "(EventLabel, Core, State) event \<Rightarrow> (State rgformula) option"
+  where "evtrgffun \<equiv> (\<lambda>e. Some (SOME rg. (e, rg)\<in>evtrgfset))"
+
+lemma evtrgffun_exist: "\<forall>e\<in>Domain evtrgfset. \<exists>ef\<in>evtrgfset. E\<^sub>e ef = e \<and> evtrgffun e = Some (snd ef)"
+  by (metis Domain_iff E\<^sub>e_def evtrgffun_def fst_conv snd_conv someI_ex)
+
+lemma diff_e_in_evtrgfset: "\<forall>ef1 ef2. ef1\<in>evtrgfset \<and> ef2\<in>evtrgfset \<and> ef1\<noteq>ef2 \<longrightarrow> E\<^sub>e ef1 \<noteq> E\<^sub>e ef2"
+  apply(rule allI)+
+  apply(case_tac "ef1\<in>(\<Union>k.{(Core_Init k, Core_Init_RGCond)})")
+    apply(case_tac "ef2 \<in> (\<Union>k. {(Core_Init k, Core_Init_RGCond)})")
+    apply(clarify) using neq_coreinit_sched apply (simp add: E\<^sub>e_def) 
+    apply(case_tac "ef2 \<in> (\<Union>k.{(Schedule k, Schedule_RGCond k)})")
+    apply(clarify) using neq_coreinit_sched apply (simp add:E\<^sub>e_def)
+    apply(case_tac "ef2 \<in> (\<Union>(k, p, m).{(Write_Sampling_Message k p m, Write_Sampling_Message_RGCond k p m)})")
+    apply(clarify) using neq_coreinit_wrtsamp apply (simp add:E\<^sub>e_def)
+    apply(case_tac "ef2 \<in> (\<Union>(k, p).{(Read_Sampling_Message k p, Read_Sampling_Message_RGCond k p)})")
+    apply(clarify) using neq_coreinit_rdsamp apply (simp add:E\<^sub>e_def)
+    using evtrgfset_def apply blast
+  apply(case_tac "ef1 \<in> (\<Union>k.{(Schedule k, Schedule_RGCond k)})")
+    apply(case_tac "ef2 \<in> (\<Union>k. {(Core_Init k, Core_Init_RGCond)})")
+    apply(clarify) using neq_coreinit_sched apply (metis E\<^sub>e_def fst_conv)
+    apply(case_tac "ef2 \<in> (\<Union>k.{(Schedule k, Schedule_RGCond k)})")
+    apply(clarify) using neq_schedule apply (metis E\<^sub>e_def fst_conv)
+    apply(case_tac "ef2 \<in> (\<Union>(k, p, m).{(Write_Sampling_Message k p m, Write_Sampling_Message_RGCond k p m)})")
+    apply(clarify) using neq_sched_wrtsamp apply (simp add: E\<^sub>e_def)
+    apply(case_tac "ef2 \<in> (\<Union>(k, p).{(Read_Sampling_Message k p, Read_Sampling_Message_RGCond k p)})")
+    apply(clarify) using neq_sched_rdsamp apply (simp add: E\<^sub>e_def)
+    apply(simp add: evtrgfset_def)
+  apply(case_tac "ef1 \<in> (\<Union>(k, p, m).{(Write_Sampling_Message k p m, Write_Sampling_Message_RGCond k p m)})")
+     apply(case_tac "ef2 \<in> (\<Union>k. {(Core_Init k, Core_Init_RGCond)})")
+    apply(clarify) using neq_coreinit_wrtsamp apply (metis (no_types, opaque_lifting) E\<^sub>e_def prod.sel(1))
+    apply(case_tac "ef2 \<in> (\<Union>k.{(Schedule k, Schedule_RGCond k)})")
+    apply(clarify) using neq_sched_wrtsamp apply (metis (no_types, opaque_lifting) E\<^sub>e_def prod.sel(1))
+    apply(case_tac "ef2 \<in> (\<Union>(k, p, m).{(Write_Sampling_Message k p m, Write_Sampling_Message_RGCond k p m)})")
+    apply(clarify) using neq_wrt_samp apply (metis (no_types, opaque_lifting) E\<^sub>e_def prod.sel(1))
+    apply(case_tac "ef2 \<in> (\<Union>(k, p).{(Read_Sampling_Message k p, Read_Sampling_Message_RGCond k p)})")
+    apply(clarify) using neq_wrtsamp_rdsamp apply (metis (no_types, opaque_lifting) E\<^sub>e_def prod.sel(1))
+    apply(simp add: evtrgfset_def)
+  apply(case_tac "ef1 \<in> (\<Union>(k, p).{(Read_Sampling_Message k p, Read_Sampling_Message_RGCond k p)})")
+    apply(case_tac "ef2 \<in> (\<Union>k. {(Core_Init k, Core_Init_RGCond)})")
+    apply(clarify) using neq_coreinit_rdsamp apply (metis (no_types, opaque_lifting) E\<^sub>e_def prod.sel(1))
+    apply(case_tac "ef2 \<in> (\<Union>k.{(Schedule k, Schedule_RGCond k)})")
+    apply(clarify) using neq_sched_rdsamp apply (metis (no_types, opaque_lifting) E\<^sub>e_def prod.sel(1))
+    apply(case_tac "ef2 \<in> (\<Union>(k, p, m).{(Write_Sampling_Message k p m, Write_Sampling_Message_RGCond k p m)})")
+    apply(clarify) using neq_wrtsamp_rdsamp apply (metis (no_types, opaque_lifting) E\<^sub>e_def prod.sel(1))
+    apply(case_tac "ef2 \<in> (\<Union>(k, p).{(Read_Sampling_Message k p, Read_Sampling_Message_RGCond k p)})")
+    apply(clarify) using neq_rd_samp apply (metis (no_types, opaque_lifting) E\<^sub>e_def prod.sel(1))
+    by(simp add: evtrgfset_def)+
+
+lemma evtrgfset_func: "\<forall>ef\<in>evtrgfset. evtrgffun (E\<^sub>e ef) = Some (snd ef)" 
+  proof -
+  {
+    fix ef
+    assume a0: "ef\<in>evtrgfset"
+    then have "E\<^sub>e ef\<in>Domain evtrgfset" by (metis Domain_iff E\<^sub>e_def surjective_pairing) 
+    then obtain ef1 where a1: "ef1\<in>evtrgfset \<and> E\<^sub>e ef1 = E\<^sub>e ef \<and> evtrgffun (E\<^sub>e ef) = Some (snd ef1)" 
+      using evtrgffun_exist[rule_format,of "E\<^sub>e ef"] by auto
+    have "evtrgffun (E\<^sub>e ef) = Some (snd ef)"
+      proof(cases "ef1 = ef")
+        assume "ef1 = ef"
+        with a1 show ?thesis by simp
+      next
+        assume b0: "ef1\<noteq>ef"
+        with diff_e_in_evtrgfset a0 a1 have "E\<^sub>e ef1 \<noteq> E\<^sub>e ef" by blast
+        with a1 show ?thesis by simp
+      qed
+  }
+  then show ?thesis by auto
+qed
+
+lemma all_basic_evts_arinc_help: "\<forall>k. ef\<in>all_evts_es (fst (ARINCXKernel_Spec k)) \<longrightarrow> is_basicevt (E\<^sub>e ef)"
+  proof -
+  {
+    fix k
+    assume p0: "ef\<in>all_evts_es (fst (ARINCXKernel_Spec k))" 
+    then have "ef\<in>all_evts_es (fst (EvtSys_on_Core_RGF k))" by (simp add:ARINCXKernel_Spec_def)
+    then have "ef\<in>insert (Core_Init_RGF k) (all_evts_es (fst (EvtSys1_on_Core_RGF k)))" 
+      by (simp add:EvtSys_on_Core_RGF_def)
+    then have "ef = (Core_Init_RGF k) \<or> ef\<in>all_evts_es (fst (EvtSys1_on_Core_RGF k))" by auto
+    then have "is_basicevt (E\<^sub>e ef)"
+      proof
+        assume a0: "ef = Core_Init_RGF k"
+        then show ?thesis 
+          using Core_Init_RGF_def Core_Init_def by (metis E\<^sub>e_def fst_conv is_basicevt.simps(2)) 
+      next
+        assume a1: "ef\<in>all_evts_es (fst (EvtSys1_on_Core_RGF k))"
+        then have "ef\<in>{Schedule_RGF k} \<union>
+                      {ef. \<exists>p m. ef = Write_Sampling_Message_RGF k p m} \<union>
+                      {ef. \<exists>p. ef = Read_Sampling_Message_RGF k p}" 
+          using all_evts_es_esys EvtSys1_on_Core_RGF_def by auto
+        then have "ef\<in>{Schedule_RGF k} 
+                  \<or> ef\<in>{ef. \<exists>p m. ef = Write_Sampling_Message_RGF k p m} 
+                  \<or> ef\<in>{ef. \<exists>p. ef = Read_Sampling_Message_RGF k p}" by auto
+        then show ?thesis
+          proof
+            assume "ef\<in>{Schedule_RGF k}"
+            then show ?thesis by (simp add: E\<^sub>e_def Schedule_RGF_def Schedule_def) 
+          next
+            assume "ef\<in>{ef. \<exists>p m. ef = Write_Sampling_Message_RGF k p m}
+                    \<or> ef\<in>{ef. \<exists>p. ef = Read_Sampling_Message_RGF k p}"
+            then show ?thesis 
+              proof
+                assume "ef\<in>{ef. \<exists>p m. ef = Write_Sampling_Message_RGF k p m}"
+                then have "\<exists>p m. ef = Write_Sampling_Message_RGF k p m" by auto
+                then obtain p and m where "ef = Write_Sampling_Message_RGF k p m" by auto
+                then show ?thesis by (simp add: E\<^sub>e_def Write_Sampling_Message_RGF_def Write_Sampling_Message_def)
+              next
+                assume "ef\<in>{ef. \<exists>p. ef = Read_Sampling_Message_RGF k p}"
+                then have "\<exists>p. ef = Read_Sampling_Message_RGF k p" by auto
+                then obtain p where "ef = Read_Sampling_Message_RGF k p" by auto
+                then show ?thesis by (simp add: E\<^sub>e_def Read_Sampling_Message_RGF_def Read_Sampling_Message_def) 
+              qed
+          qed
+      qed
+  }
+  then show ?thesis by auto
+  qed
+
+lemma all_basic_evts_arinc: "\<forall>ef\<in>all_evts ARINCXKernel_Spec. is_basicevt (E\<^sub>e ef)" 
+  using all_evts_def[of ARINCXKernel_Spec] all_basic_evts_arinc_help by auto
+
+lemma bsc_evts_rgfs: "\<forall>erg\<in>all_evts (ARINCXKernel_Spec). (evtrgffun (E\<^sub>e erg))  = Some (snd erg)"
+  using evtrgfset_func evtrgfset_eq_allevts_ARINCSpec by simp
+
+interpretation RG_InfoFlow C0 exec_step interf state_equiv state_obs domevt 
+  ARINCXKernel_Spec s0 x0 evtrgffun "paresys_spec ARINCXKernel_Spec"
+    using state_equiv_transitive state_equiv_reflexive state_equiv_symmetric exec_step_def 
+      C0_init all_basic_evts_arinc bsc_evts_rgfs spec_sat_rg
+    InfoFlow.intro[of state_equiv exec_step domevt]
+    RG_InfoFlow.intro[of exec_step state_equiv domevt C0 ARINCXKernel_Spec 
+                        s0 x0 evtrgffun "paresys_spec ARINCXKernel_Spec"]
+    RG_InfoFlow_axioms.intro[of C0 ARINCXKernel_Spec s0 x0 "paresys_spec ARINCXKernel_Spec" evtrgffun]  
+    by (metis (no_types, lifting) option.sel)
+
+lemma s0_update_help: "\<lbrakk>schan1 = schan2; recv1 = recv2 \<rbrakk> \<Longrightarrow> 
+                      s0\<lparr> schan := schan1, recv := recv1\<rparr> = s0\<lparr> schan := schan2, recv := recv2\<rparr>"
+  by blast
+
+
+lemma Core_Init_sat_SCE: "\<exists>\<S>. Core_Init k \<in> \<S> \<and> step_consistent_e \<S> (Core_Init k)"
+  apply (rule sc_e_Basic, simp add: Core_Init_def)
+  by (simp add: body_def  sc_p.Basic)
+
+lemma Schedule_sat_SCE: "\<exists>\<S>. Schedule k \<in> \<S> \<and> step_consistent_e \<S> (Schedule k)"
+  apply (rule sc_e_Basic, simp add: Schedule_def)
+  apply (simp add: body_def)
+  apply (rule sc_p.Basic, clarsimp)
+  apply (case_tac u)
+   apply (simp add: state_equiv_def state_obs_part_def schan_obs_part_def)
+  by ( simp add: state_equiv_def state_obs_sched_def)
+
+lemma Read_Sampling_sat_SCE: "\<exists>\<S>. Read_Sampling_Message k p \<in> \<S> \<and> step_consistent_e \<S> (Read_Sampling_Message k p)"
+  apply (rule sc_e_Basic, simp add: Read_Sampling_Message_def)
+  apply (simp add: body_def)
+  apply (rule sc_p.Basic, clarsimp)
+  apply (case_tac u)
+  apply (case_tac "ka = k", simp)
+    apply (case_tac "x1 = (cur s1) (gsch conf k)")
+     apply (erule impE)
+      apply (metis domevt_def interf_def) 
+     apply (simp add: state_equiv_def state_obs_part_def schan_obs_part_def, clarify)
+     apply (rule s0_update_help)
+      apply (simp add: System_Init_def s0_init)
+     apply (metis (no_types, lifting) State.ext_inject State.update_convs(2) State.update_convs(3) 
+            System_Init_def ch_destsampport_same prod.sel(1) s0_init schan_obs_part_def)
+    apply (simp add: port_of_part_def schan_obs_part_def state_equiv_def state_obs_part_def)
+   apply (simp add: state_equiv_def state_obs_part_def schan_obs_part_def, clarify)
+   apply (rule s0_update_help, simp add: System_Init_def s0_init)
+   apply (metis (no_types, lifting) State.ext_inject State.update_convs(2) State.update_convs(3) 
+      System_Init_def ch_destsampport_same port_of_part_def prod.sel(1) s0_init schan_obs_part_def)
+  by (simp add: state_equiv_def state_obs_sched_def)
+
+lemma Write_Sampling_sat_SCE: "\<exists>\<S>. Write_Sampling_Message k p m \<in> \<S> \<and> step_consistent_e \<S> (Write_Sampling_Message k p m)"
+  apply (rule sc_e_Basic, simp add: Write_Sampling_Message_def)
+  apply (simp add: body_def)
+  apply (rule sc_p.Basic, clarsimp)
+  apply (case_tac u)
+   apply (simp add: state_equiv_def state_obs_part_def schan_obs_part_def, clarify)
+   apply (rule s0_update_help)
+    apply (metis (no_types, lifting) State.ext_inject State.update_convs(2) State.update_convs(3) 
+       System_Init_def fun_upd_restrict_conv prod.sel(1) s0_init)
+   apply (simp add: System_Init_def s0_init)
+  by(simp add: state_equiv_def state_obs_sched_def)
+
+lemma Core_Init_sat_LRE: 
+  "\<forall>u s1 s2 x. (s1,s2) \<in> Guar\<^sub>f Core_Init_RGCond 
+                \<longrightarrow> ((domevt s1 k (Core_Init x)) \<setminus>\<leadsto> u \<longrightarrow> s1 \<sim>u\<sim> s2)"
+  apply (simp add: Core_Init_RGCond_def Guar\<^sub>f_def getrgformula_def, clarsimp)
+  apply (case_tac u, simp add: vpeq_reflexive)
+  using vpeq_reflexive by force
+
+lemma Schedule_sat_LRE: 
+  "\<forall>u s1 s2 x. (s1,s2) \<in> Guar\<^sub>f (Schedule_RGCond x) 
+                \<longrightarrow> ((domevt s1 k (Schedule x)) \<setminus>\<leadsto> u \<longrightarrow> s1 \<sim>u\<sim> s2)"
+  apply (simp add: Schedule_RGCond_def Guar\<^sub>f_def getrgformula_def, clarsimp)
+  apply (case_tac u, simp add: vpeq_reflexive, clarsimp)
+   apply (simp add: state_equiv_def state_obs_part_def)
+  using schan_obs_part_def apply presburger
+  apply (simp add: vpeq_reflexive, clarsimp)
+  apply (simp add: state_equiv_def state_obs_sched_def)
+  apply (simp add: domevt_def gsch_def neq_sched_rdsamp neq_sched_wrtsamp)
+  
+  sorry
+
+
+
+lemma Read_Sampling_sat_LRE:
+  "\<forall>u s1 s2 k. (s1,s2) \<in> Guar\<^sub>f (Read_Sampling_Message_RGCond x p) 
+                \<longrightarrow> ((domevt s1 k (Read_Sampling_Message x p)) \<setminus>\<leadsto> u \<longrightarrow> s1 \<sim>u\<sim> s2)"
+  apply (simp add: Read_Sampling_Message_RGCond_def Guar\<^sub>f_def getrgformula_def, clarsimp)
+  apply (case_tac "x = k")
+  apply (case_tac u, simp add: vpeq_reflexive, clarsimp)
+   apply (case_tac "x1 = (cur s1) (gsch conf x)")
+    apply (metis domevt_def interf_def noninterf1_def)
+   apply (simp add: state_equiv_def state_obs_part_def)
+   apply (rule s0_update_help, simp add: schan_obs_part_def)
+   apply blast
+   apply (simp add: state_equiv_def state_obs_sched_def)
+  sorry
+
+lemma Write_Sampling_sat_LRE:
+  "\<forall>u s1 s2 k. (s1,s2) \<in> Guar\<^sub>f (Write_Sampling_Message_RGCond k p m) 
+                \<longrightarrow> ((domevt s1 k (Write_Sampling_Message k p m)) \<setminus>\<leadsto> u \<longrightarrow> s1 \<sim>u\<sim> s2)"
+proof-
+  {
+    fix u s1 s2 k
+    assume a0: "(s1,s2) \<in> Guar\<^sub>f (Write_Sampling_Message_RGCond k p m)"
+       and a1: "domevt s1 k (Write_Sampling_Message k p m) \<setminus>\<leadsto> u"
+    then have eq: "cur s2 = cur s1 \<and> recv s2 = recv s1 \<and> 
+    (is_src_sampport conf p \<and> port_of_part conf p ((cur s1) (c2s conf k)) \<longrightarrow>
+    (\<forall>ch. ch \<noteq> (ch_srcsampport conf p) \<longrightarrow> (schan s1) ch = (schan s2) ch)) \<and> 
+    (\<not> (is_src_sampport conf p \<and> port_of_part conf p ((cur s1) (c2s conf k))) \<longrightarrow>
+    schan s1 = schan s2)"
+      using a0 unfolding Write_Sampling_Message_RGCond_def Guar\<^sub>f_def getrgformula_def 
+      by auto
+    then have "s1 \<sim>u\<sim> s2"
+    proof-
+      {
+        assume pre_cond: "is_src_sampport conf p \<and> port_of_part conf p ((cur s1) (c2s conf k))"
+        have "domevt s1 k (Write_Sampling_Message k p m) = P ((cur s1) (c2s conf k))"
+          using domevt_def gsch_def by auto
+      then have non_inter:"P ((cur s1) (c2s conf k)) \<noteq> u \<and> 
+              \<not>(part_on_core conf u (P ((cur s1) (c2s conf k)) )) \<and> 
+              \<not>ch_conn2 conf (P ((cur s1) (c2s conf k))) u" 
+        by (metis a1 interf_def noninterf1_def)
+      then have "(\<exists>d1. u = S d1) \<or> (\<exists>d1. u=P d1)"
+        by (metis Domain.exhaust)
+      then have ?thesis
+      proof
+        assume "\<exists>d1. u = S d1"
+        thus ?thesis
+          using eq state_equiv_def state_obs_sched_def by force
+      next
+        assume u:"\<exists>d1. u=P d1"
+        then obtain d1 where u:"u=P d1" by auto
+        then have d1_not_cur_core:"d1 \<noteq> ((cur s1) (c2s conf k))"
+          using non_inter by blast
+        then have "(\<exists>d1. u= S d1) \<or> \<not>ch_conn conf ((cur s1) (c2s conf k)) d1"
+          using non_inter u by auto
+        thus ?thesis
+        proof
+          assume "\<exists>d1. u = S d1" thus ?thesis using u by auto
+        next
+          assume a0:"\<not>ch_conn conf ((cur s1) (c2s conf k)) d1"   
+          then have a0:"(\<forall>sch p. (p2p conf (scsrc conf sch) = cur s1 (c2s conf k)) \<longrightarrow> 
+                  \<not>(p \<in> scdests conf sch \<and> p2p conf p = d1))"
+            unfolding ch_conn_def by auto
+          obtain ch where  eq_schan:"ch =(ch_srcsampport conf p) \<and>  
+            (\<forall>ch'. (ch'\<noteq>ch \<longrightarrow> (schan s2) ch' = (schan s1) ch'))"
+            using eq by fastforce
+          have "ch \<notin>(par_sampchan conf d1)"
+          proof 
+            assume ch_par:"ch \<in> (par_sampchan conf d1)"
+            then have "ch \<in> (ch_srcsampport conf) ` (par_src_sampling_ports conf (par_ports conf d1)) \<or>
+                    ch \<in> (ch_destsampport conf) `(par_dest_sampling_ports conf (par_ports conf d1))"
+              using a0 unfolding par_sampchan_def by auto  
+            then show False
+              unfolding par_sampchan_def ch_srcsampport_def
+              using  a0 d1_not_cur_core pre_cond eq_schan  ch_par port_disj scdests_not_emp no_disconn_port  
+                    no_same_source no_same_dest bij_p2p    
+              unfolding  ch_srcsampport_def par_src_sampling_ports_def par_ports_def port_of_part_def
+                  is_src_sampport_def par_dest_sampling_ports_def is_dest_sampport_def
+                  image_def ch_destsampport_def par_sampchan_def gsch_def 
+              apply auto
+               apply (metis (mono_tags))
+              by (metis (mono_tags, lifting))
+          qed
+          then have "\<forall>ch \<in>(par_sampchan conf d1). (schan s2) ch = (schan s1) ch" 
+            using eq_schan by force 
+          then have "schan_obs_part s1 d1 = schan_obs_part s2 d1" 
+            unfolding  schan_obs_part_def restrict_map_def by auto
+          then have "state_obs_part s1 d1 = state_obs_part s2 d1"  
+            unfolding state_obs_part_def
+            using eq by auto      
+          thus ?thesis using u unfolding state_equiv_def by auto  
+        qed        
+      qed
+    } note l=this
+     {assume "\<not> is_src_sampport conf p \<and> port_of_part conf p ((cur s1) (c2s conf k))"
+      then have "cur s2= cur s1 \<and> schan s2 = schan s1"
+        using eq by auto
+      then have "s1 = s2" 
+        by (simp add: eq)
+      then have "s1 \<sim>u\<sim> s2" 
+        unfolding state_equiv_def by auto
+    } 
+    thus ?thesis using eq l 
+      by (metis State.surjective old.unit.exhaust vpeq_reflexive)
+  qed
+}thus ?thesis by auto
+qed
+
+
+lemma uwce_LRE_help: "\<forall>x. ef \<in> all_evts_es (fst (ARINCXKernel_Spec x)) \<and> (s1,s2) \<in> Guar\<^sub>e ef \<longrightarrow> 
+                                    ((domevt s1 k (E\<^sub>e ef)) \<setminus>\<leadsto> u \<longrightarrow> s1 \<sim>u\<sim> s2)"
+  proof -
+  {
+    fix x
+    assume p0: "ef\<in>all_evts_es (fst (ARINCXKernel_Spec x))" 
+    then have "ef\<in>all_evts_es (fst (EvtSys_on_Core_RGF x))" by (simp add:ARINCXKernel_Spec_def)
+    then have "ef\<in>insert (Core_Init_RGF x) (all_evts_es (fst (EvtSys1_on_Core_RGF x)))" 
+      by (simp add:EvtSys_on_Core_RGF_def)
+    then have "ef = (Core_Init_RGF x) \<or> ef\<in>all_evts_es (fst (EvtSys1_on_Core_RGF x))" by auto
+    then have "(s1,s2) \<in> Guar\<^sub>e ef \<longrightarrow> ((domevt s1 k (E\<^sub>e ef)) \<setminus>\<leadsto> u \<longrightarrow> s1 \<sim>u\<sim> s2)"
+      proof
+        assume a0: "ef = Core_Init_RGF x"
+        then show ?thesis
+          by (simp add: Core_Init_RGF_def Core_Init_sat_LRE E\<^sub>e_def Guar\<^sub>e_def Guar\<^sub>f_def)          
+      next
+        assume a1: "ef\<in>all_evts_es (fst (EvtSys1_on_Core_RGF x))"
+        then have "ef\<in>{Schedule_RGF x} \<union>
+                      {ef. \<exists>p m. ef = Write_Sampling_Message_RGF x p m} \<union>
+                      {ef. \<exists>p. ef = Read_Sampling_Message_RGF x p}" 
+          using all_evts_es_esys EvtSys1_on_Core_RGF_def by auto
+        then have "ef\<in>{Schedule_RGF x} 
+                  \<or> ef\<in>{ef. \<exists>p m. ef = Write_Sampling_Message_RGF x p m} 
+                  \<or> ef\<in>{ef. \<exists>p. ef = Read_Sampling_Message_RGF x p}" by auto
+        then show ?thesis
+          proof
+            assume "ef\<in>{Schedule_RGF x}"
+            then show ?thesis 
+              by (simp add: E\<^sub>e_def Guar\<^sub>e_def Guar\<^sub>f_def Schedule_RGF_def Schedule_sat_LRE) 
+          next
+            assume "ef\<in>{ef. \<exists>p m. ef = Write_Sampling_Message_RGF k p m}
+                    \<or> ef\<in>{ef. \<exists>p. ef = Read_Sampling_Message_RGF k p}"
+            then show ?thesis 
+              proof
+                assume "ef\<in>{ef. \<exists>p m. ef = Write_Sampling_Message_RGF k p m}"
+                then have "\<exists>p m. ef = Write_Sampling_Message_RGF k p m" by auto
+                then obtain p and m where "ef = Write_Sampling_Message_RGF k p m" by auto
+                then show ?thesis 
+                  by (simp add: E\<^sub>e_def Guar\<^sub>e_def Guar\<^sub>f_def Write_Sampling_Message_RGF_def Write_Sampling_sat_LRE)
+              next
+                assume "ef\<in>{ef. \<exists>p. ef = Read_Sampling_Message_RGF k p}"
+                then have "\<exists>p. ef = Read_Sampling_Message_RGF k p" by auto
+                then obtain p where "ef = Read_Sampling_Message_RGF k p" by auto
+                then show ?thesis 
+                  by (simp add: E\<^sub>e_def Guar\<^sub>e_def Guar\<^sub>f_def Read_Sampling_Message_RGF_def Read_Sampling_sat_LRE)
+              qed
+          qed
+      qed
+  }
+  then show ?thesis sorry
+qed
+
+
+lemma uwce_SCE_help: "\<forall>k. ef \<in> all_evts_es (fst (ARINCXKernel_Spec k)) \<longrightarrow> (\<exists>\<S>. E\<^sub>e ef \<in> \<S> \<and> step_consistent_e \<S> (E\<^sub>e ef))"
+  proof -
+  {
+    fix k
+    assume p0: "ef\<in>all_evts_es (fst (ARINCXKernel_Spec k))" 
+    then have "ef\<in>all_evts_es (fst (EvtSys_on_Core_RGF k))" by (simp add:ARINCXKernel_Spec_def)
+    then have "ef\<in>insert (Core_Init_RGF k) (all_evts_es (fst (EvtSys1_on_Core_RGF k)))" 
+      by (simp add:EvtSys_on_Core_RGF_def)
+    then have "ef = (Core_Init_RGF k) \<or> ef\<in>all_evts_es (fst (EvtSys1_on_Core_RGF k))" by auto
+    then have "\<exists>\<S>. E\<^sub>e ef \<in> \<S> \<and> step_consistent_e \<S> (E\<^sub>e ef)"
+      proof
+        assume a0: "ef = Core_Init_RGF k"
+        then show ?thesis 
+          by (simp add: Core_Init_RGF_def Core_Init_sat_SCE E\<^sub>e_def)  
+      next
+        assume a1: "ef\<in>all_evts_es (fst (EvtSys1_on_Core_RGF k))"
+        then have "ef\<in>{Schedule_RGF k} \<union>
+                      {ef. \<exists>p m. ef = Write_Sampling_Message_RGF k p m} \<union>
+                      {ef. \<exists>p. ef = Read_Sampling_Message_RGF k p}" 
+          using all_evts_es_esys EvtSys1_on_Core_RGF_def by auto
+        then have "ef\<in>{Schedule_RGF k} 
+                  \<or> ef\<in>{ef. \<exists>p m. ef = Write_Sampling_Message_RGF k p m} 
+                  \<or> ef\<in>{ef. \<exists>p. ef = Read_Sampling_Message_RGF k p}" by auto
+        then show ?thesis
+          proof
+            assume "ef\<in>{Schedule_RGF k}"
+            then show ?thesis 
+              by (simp add: E\<^sub>e_def Schedule_RGF_def Schedule_sat_SCE) 
+          next
+            assume "ef\<in>{ef. \<exists>p m. ef = Write_Sampling_Message_RGF k p m}
+                    \<or> ef\<in>{ef. \<exists>p. ef = Read_Sampling_Message_RGF k p}"
+            then show ?thesis 
+              proof
+                assume "ef\<in>{ef. \<exists>p m. ef = Write_Sampling_Message_RGF k p m}"
+                then have "\<exists>p m. ef = Write_Sampling_Message_RGF k p m" by auto
+                then obtain p and m where "ef = Write_Sampling_Message_RGF k p m" by auto
+                then show ?thesis 
+                  by (simp add: E\<^sub>e_def Write_Sampling_Message_RGF_def Write_Sampling_sat_SCE)
+              next
+                assume "ef\<in>{ef. \<exists>p. ef = Read_Sampling_Message_RGF k p}"
+                then have "\<exists>p. ef = Read_Sampling_Message_RGF k p" by auto
+                then obtain p where "ef = Read_Sampling_Message_RGF k p" by auto
+                then show ?thesis 
+                  by (simp add: E\<^sub>e_def Read_Sampling_Message_RGF_def Read_Sampling_sat_SCE)
+              qed
+          qed
+      qed
+  }
+  then show ?thesis by auto
+qed
+
+theorem uwc_oc: "observed_consistent"
+  apply(simp add:observed_consistent_def)
+  by(simp add:state_equiv_def)
+
+
+theorem uwce_LRE: "locally_respect_events_guar"
+  apply (simp add: locally_respect_events_guar_def all_evts_def, clarify)
+  using all_evts_def[of ARINCXKernel_Spec] uwce_LRE_help 
+  using noninterf1_def noninterf_def by blast
+                                               
+
+theorem uwce_SCE: "step_consistent_events"
+  apply (simp add: step_consistent_events_def)
+  using all_evts_def[of ARINCXKernel_Spec] uwce_SCE_help by auto
+
+
+theorem "noninfluence0"
+  using uwc_oc uwce_LRE uwce_SCE UnwindingTheoremE_noninfluence0_guar by simp
+
+theorem "nonleakage"
+  using UnwindingTheorem_nonleakage rg_lr_guar_imp_lr rg_sc_imp_sc uwc_oc uwce_LRE uwce_SCE by blast
 
 
 
